Part of the preservation of typing

src/Lustre/Normalization/Correctness.v
@@ -1,4 +1,6 @@
 From Coq Require Import List.
+Import List.ListNotations.
+Open Scope list_scope.
 
 From Velus Require Import Common Ident.
 From Velus Require Import Operators Environment.
@@ -21,34 +23,165 @@ Module Type CORRECTNESS
        (Import Norm : NORMALIZATION Ids Op OpAux Syn Typ).
   Import List.
 
+  Definition st_tys (st : fresh_st (ann * bool)) := idty (idty (snd st)).
+
+  Fact st_follows_tys_incl : forall st st',
+      fresh_st_follows st st' ->
+      incl (st_tys st) (st_tys st').
+  Proof.
+    intros st st' [Hincl _].
+    unfold incl in *. intros [id data] Hin.
+    unfold st_tys, idty in *.
+    repeat simpl_In. inv H. inv H0.
+    exists (id, (data, n)). split; auto.
+    repeat simpl_In.
+    exists (id, (data, n, b)). eauto.
+  Qed.
+
+  Fact idents_for_anns_incl : forall anns ids st st',
+      idents_for_anns anns st = (ids, st') ->
+      incl ids (idty (snd st')).
+  Proof.
+    induction anns; intros ids st st' Hids; simpl in Hids; repeat inv_bind;
+      unfold incl; intros ? Hin; inv Hin.
+    - unfold fresh_ident in H; destruct st as [n l]; inv H.
+      apply idents_for_anns_st_follows in H0; destruct H0 as [Hfollows _].
+      unfold idty. simpl_In.
+      exists (x, (a, false)); simpl. split; auto.
+      apply Hfollows. simpl. auto.
+    - apply IHanns in H0; auto.
+  Qed.
+
+  Ltac solve_incl :=
+    match goal with
+    | H : wt_clock ?l1 ?cl |- wt_clock ?l2 ?cl =>
+      eapply wt_clock_incl; [| eauto]
+    | H : wt_nclock ?l1 ?cl |- wt_nclock ?l2 ?cl =>
+      eapply wt_nclock_incl; [| eauto]
+    | H : wt_exp ?G ?l1 ?e |- wt_exp ?G ?l2 ?e =>
+      eapply wt_exp_incl; [| eauto]
+    | H : wt_equation ?G ?l1 ?eq |- wt_equation ?G ?l2 ?eq =>
+      eapply wt_equation_incl; [| eauto]
+    | |- incl ?l1 ?l1 => reflexivity
+    | |- incl ?l1 (?l1 ++ ?l2) =>
+      eapply incl_appl; reflexivity
+    | |- incl (?l1 ++ ?l2) (?l1 ++ ?l3) =>
+      eapply incl_app
+    | |- incl ?l1 (?l2 ++ ?l3) =>
+      eapply incl_appr
+    | |- incl (st_tys ?st1) (st_tys _) =>
+      eapply st_follows_tys_incl; repeat solve_st_follows
+    | H : incl ?l1 ?l2 |- incl (idty ?l1) (idty ?l2) =>
+      eapply incl_map; eauto
+    end.
+
   Ltac singleton_length :=
     simpl in *;
     match goal with
     | H : length ?x = 1 |- _ =>
-      destruct x; simpl in H; try congruence;
-      destruct x; simpl in H; try congruence;
-      simpl in *; clear H
+      destruct x; simpl in *; try congruence
+    end;
+    match goal with
+    | H : S (length ?x) = 1 |- _ =>
+      destruct x; simpl in *; try congruence;
+      clear H
     end.
 
-  Fact map_bind2_wt_exp {A A2 B} :
-    forall G vars (k : A -> Fresh (list exp * A2) B) a es' a2s st st',
-      map_bind2 k a st = (es', a2s, st') ->
-      Forall (fun a => forall es' a2s st st',
-                  k a st = (es', a2s, st') ->
-                  Forall (wt_exp G vars) es') a ->
-      Forall (wt_exp G vars) (concat es').
+  Ltac subst_length :=
+    match goal with
+    | H: length ?x1 = length ?x2 |- context l [length ?x1] =>
+      rewrite H
+    | H: length ?x1 = length ?x2, H1: context l [length ?x1] |- _ =>
+      rewrite H in H1
+    | H: ?x1 = ?x2 |- context l [length ?x1] =>
+      rewrite H
+    | H: ?x1 = ?x2, H1: context l [length ?x1] |- _ =>
+      rewrite H in H1
+    end.
+
+  Ltac simpl_length :=
+    repeat subst_length;
+    (match goal with
+     | H : context c [Nat.min ?x1 ?x1] |- _ =>
+       repeat rewrite PeanoNat.Nat.min_id in H
+     | H : context c [length (combine _ _)] |- _ =>
+       rewrite combine_length in H
+     | H : context c [length (map _ _)] |- _ =>
+       rewrite map_length in H
+     | |- context c [Nat.min ?x1 ?x1] =>
+       rewrite PeanoNat.Nat.min_id
+     | |- context c [length (combine _ _)] =>
+       rewrite combine_length
+     | |- context c [length (map _ _)] =>
+       rewrite map_length
+    end).
+
+  Ltac solve_length :=
+    repeat simpl_length; solve [auto].
+
+  Ltac simpl_nth :=
+    match goal with
+    | H : In ?x _ |- _ =>
+      apply In_nth with (d:=x) in H; destruct H as [? [? ?]]; try simpl_nth
+    | H : nth _ (combine _ _) _ = _ |- _ =>
+      rewrite combine_nth in H; [inv H; try simpl_nth|repeat solve_length]
+    end.
+
+  Hint Resolve in_combine_l in_combine_r.
+  Hint Resolve incl_tl incl_appl incl_appr incl_app incl_refl.
+
+  Fact normalize_exp_numstreams : forall e is_control es' eqs' st st',
+      normalize_exp is_control e st = (es', eqs', st') ->
+      Forall (fun e => numstreams e = 1) es'.
   Proof.
-    intros G vars k a es' a2s st st' Hmap Hf.
-    apply map_bind2_values in Hmap.
-    induction Hmap; inv Hf.
-    - constructor.
-    - simpl. apply Forall_app.
-      destruct H as [? [? H]].
-      split; eauto.
+    intros e is_control es' eqs' st st' Hnorm.
+    induction e; simpl in Hnorm; repeat inv_bind; repeat constructor.
+    2: destruct l0.
+    3,4: destruct l1.
+    3,4: destruct is_control.
+    1,2,3,4,5,6,7:(repeat inv_bind; rewrite Forall_forall; intros ? Hin;
+                   repeat simpl_In; reflexivity).
   Qed.
 
-  (** ** Preservation of good typing
-      TODO is this necessary ? *)
+  Corollary map_bind2_normalize_exp_numstreams : forall es is_control es' eqs' st st',
+      map_bind2 (normalize_exp is_control) es st = (es', eqs', st') ->
+      Forall (fun e => numstreams e = 1) (concat es').
+  Proof.
+    intros es is_control es' eqs' st st' Hmap.
+    apply map_bind2_values in Hmap.
+    induction Hmap; simpl.
+    - constructor.
+    - apply Forall_app; split; auto.
+      destruct H as [? [? H]].
+      eapply normalize_exp_numstreams; eauto.
+  Qed.
+
+  Corollary normalize_exps_numstreams : forall es es' eqs' st st',
+      normalize_exps es st = (es', eqs', st') ->
+      Forall (fun e => numstreams e = 1) es'.
+  Proof.
+    intros es es' eqs' st st' Hnorm.
+    unfold normalize_exps in Hnorm. repeat inv_bind.
+    eapply map_bind2_normalize_exp_numstreams. eauto.
+  Qed.
+
+  Fact normalize_fby_numstreams : forall e0s es anns es' eqs' st st',
+      normalize_fby e0s es anns st = (es', eqs', st') ->
+      Forall (fun e => numstreams e = 1) es'.
+  Proof.
+    intros e0s es anns es' eqs' st st' Hnorm.
+    unfold normalize_fby in Hnorm. repeat inv_bind.
+    apply map_bind2_values in H.
+    repeat rewrite_Forall_forall.
+    eapply In_nth with (d:=x) in H2; destruct H2 as [n [? ?]].
+    repeat simpl_length.
+    specialize (H1 (x, x, (Op.bool_type, (Cbase, None))) x [] _ _ _ _ H2 eq_refl eq_refl eq_refl).
+    destruct H1 as [st'' [st''' H1]]. destruct (nth _ _ _) as [[e0 e] [ty cl]]. rewrite <- H3.
+    specialize (fby_iteexp_spec e0 e ty cl) as [[? [? Hspec]]|Hspec]; subst;
+      rewrite Hspec in H1; clear Hspec; repeat inv_bind; reflexivity.
+  Qed.
+
+  (** ** Preservation of wt *)
 
   Fact idents_for_anns_wt : forall G vars anns ids st st',
       idents_for_anns anns st = (ids, st') ->
@@ -63,46 +196,204 @@ Module Type CORRECTNESS
       econstructor; eauto.
       + repeat constructor; simpl; auto.
         * apply in_or_app. right. constructor; auto.
-        * eapply wt_nclock_incl; eauto.
-          apply incl_appl. reflexivity.
+        * eapply wt_nclock_incl; [| eauto]. eauto.
       + eapply Forall_impl; [| eauto].
-        intros. eapply wt_exp_incl; eauto.
-        apply incl_app.
-        * apply incl_appl. reflexivity.
-        * apply incl_appr. apply incl_tl. reflexivity.
+        intros. eapply wt_exp_incl; [| eauto]. eauto.
   Qed.
 
-  Fact st_follows_incl {A1 A2 A3} : forall (st st' : fresh_st ((A1 * A2) * A3)),
-      fresh_st_follows st st' ->
-      incl (idty (idty (snd st))) (idty (idty (snd st'))).
+  Fact hd_default_wt_exp : forall G vars es,
+      Forall (wt_exp G vars) es ->
+      wt_exp G vars (hd_default es).
   Proof.
-    intros st st' [Hincl _].
-    unfold incl in *. intros [id data] Hin.
-    unfold idty in *.
-    rewrite in_map_iff in *. destruct Hin as [x [H Hin]]; subst. inv H.
-    exists x. split; auto.
-    rewrite in_map_iff in *. destruct Hin as [x' [H Hin]]; subst.
-    exists x'. eauto.
+    intros G vars es Hf.
+    destruct es; simpl.
+    - constructor.
+    - inv Hf; auto.
+  Qed.
+
+  Fact map_bind2_wt_exp' {A A2 B} :
+    forall G vars (k : A -> Fresh (exp * A2) B) a es' a2s st st',
+      map_bind2 k a st = (es', a2s, st') ->
+      (forall st st' a es a2s, k a st = (es, a2s, st') -> fresh_st_follows st st') ->
+      Forall (fun a => forall e' a2s st0 st0',
+                  k a st0 = (e', a2s, st0') ->
+                  fresh_st_follows st st0 ->
+                  fresh_st_follows st0' st' ->
+                  wt_exp G vars e') a ->
+      Forall (wt_exp G vars) es'.
+  Proof.
+    intros G vars k a.
+    induction a; intros es' a2s st st' Hmap Hfollows Hforall;
+      simpl in Hmap; repeat inv_bind.
+    - constructor.
+    - constructor.
+      + rewrite Forall_forall in Hforall.
+        eapply Hforall; eauto.
+        * constructor. reflexivity.
+        * reflexivity.
+        * eapply map_bind2_st_follows in H0; eauto.
+          rewrite Forall_forall; intros; eauto.
+      + eapply IHa; eauto.
+        rewrite Forall_forall in *; intros.
+        eapply Hforall; eauto. apply in_cons; auto.
+        etransitivity; eauto.
+  Qed.
+
+  Fact map_bind2_wt_exp {A A2 B} :
+    forall G vars (k : A -> Fresh (list exp * A2) B) a es' a2s st st',
+      map_bind2 k a st = (es', a2s, st') ->
+      (forall st st' a es a2s, k a st = (es, a2s, st') -> fresh_st_follows st st') ->
+      Forall (fun a => forall es' a2s st0 st0',
+                  k a st0 = (es', a2s, st0') ->
+                  fresh_st_follows st st0 ->
+                  fresh_st_follows st0' st' ->
+                  Forall (wt_exp G vars) es') a ->
+      Forall (wt_exp G vars) (concat es').
+  Proof.
+    intros G vars k a.
+    induction a; intros es' a2s st st' Hmap Hfollows Hforall;
+      simpl in Hmap; repeat inv_bind.
+    - constructor.
+    - apply Forall_app. split; eauto.
+      + rewrite Forall_forall in Hforall.
+        eapply Hforall; eauto.
+        * constructor. reflexivity.
+        * reflexivity.
+        * eapply map_bind2_st_follows in H0; eauto.
+          rewrite Forall_forall; intros; eauto.
+      + eapply IHa; eauto.
+        rewrite Forall_forall in *; intros.
+        eapply Hforall; eauto. apply in_cons; auto.
+        etransitivity; eauto.
   Qed.
 
   Hint Constructors wt_exp.
-  Fact normalize_exp_wt : forall G vars e is_control es' eqs' st st',
+
+  Fact normalize_fby_wt_exp : forall G vars e0s es anns es' eqs' st st',
+      Forall (wt_exp G (vars++(st_tys st))) e0s ->
+      Forall (wt_exp G (vars++(st_tys st))) es ->
+      Forall2 (fun e0 a => typeof e0 = [fst a]) e0s anns ->
+      Forall2 (fun e a => typeof e = [fst a]) es anns ->
+      Forall (fun '(_, cl) => wt_nclock vars cl) anns ->
+      normalize_fby e0s es anns st = (es', eqs', st') ->
+      Forall (wt_exp G (vars++(st_tys st'))) es'.
+  Proof.
+    intros G vars e0s es anns es' eqs' st st' Hwt1 Hwt2 Hty1 Hty2 Hclock Hnorm.
+    unfold normalize_fby in Hnorm. repeat inv_bind.
+    eapply map_bind2_wt_exp' in H; eauto.
+    - destruct a as [[e0 e] a]. eauto.
+    - solve_forall. destruct x as [[e0 e] [ty cl]].
+      specialize (fby_iteexp_spec e0 e ty cl) as [[? [? Hspec]]|Hspec]; subst;
+        rewrite Hspec in H1; clear Hspec; repeat inv_bind.
+      + repeat rewrite_Forall_forall.
+        repeat constructor; simpl.
+        * repeat simpl_In.
+          apply Hwt2 in H7.
+          repeat solve_incl.
+        * rewrite app_nil_r.
+          repeat rewrite_Forall_forall.
+          simpl_nth; repeat simpl_length.
+          specialize (H4 _ _ _ _ _ H0 H11 H10). simpl in H4.
+          congruence.
+        * f_equal. simpl_nth; repeat simpl_length.
+          specialize (H6 _ _ _ _ _ H0 H8 H10); simpl in H6.
+          congruence.
+        * repeat simpl_In.
+          apply Hclock in H0. repeat solve_incl.
+      + repeat rewrite_Forall_forall.
+        repeat simpl_length.
+        repeat constructor; simpl.
+        * unfold init_var_for_clock in H1. destruct st0.
+          destruct (find _ _) eqn:Hfind.
+          -- destruct p. inv H1.
+             apply find_some in Hfind; destruct Hfind as [Hfind1 Hfind2].
+             destruct p as [[? ?] ?].
+             repeat rewrite Bool.andb_true_iff in Hfind2. destruct Hfind2 as [[_ Hfind2] _].
+             rewrite equiv_decb_equiv in Hfind2.
+             apply fresh_ident_st_follows in H4.
+             assert (incl (idty (idty l)) (vars++(st_tys st'))) as Hincl.
+             { repeat solve_incl. apply st_follows_tys_incl in H4. apply st_follows_tys_incl in H3.
+               simpl in *. etransitivity; eauto. }
+             apply Hincl. repeat unfold idty; repeat simpl_In.
+             exists (x, (t, n)); simpl; auto. split.
+             ++ repeat f_equal. apply Hfind2.
+             ++ repeat simpl_In. exists (x, (t, n, b)); simpl; eauto.
+          -- inv H1.
+             assert (incl (idty(idty(snd (Pos.succ x, (x, (Op.bool_type, cl, true))::l)))) (vars++(st_tys st'))).
+             { repeat solve_incl. apply st_follows_tys_incl. repeat solve_st_follows. }
+             apply H1; simpl; auto.
+        * repeat simpl_In. apply Hclock in H0. repeat solve_incl.
+        * repeat simpl_In. apply Hwt1 in H10. repeat solve_incl.
+        * unfold fresh_ident in H4; destruct x2 as [n l]; inv H4.
+          apply st_follows_tys_incl in H3. eapply incl_appr in H3.
+          eapply H3. simpl; auto.
+        * repeat simpl_In. apply Hclock in H0. repeat solve_incl.
+        * rewrite app_nil_r.
+          simpl_nth. repeat simpl_length.
+          specialize (H8 _ _ _ _ _ H0 H10 H12). simpl in H8.
+          congruence.
+        * repeat simpl_In. apply Hclock in H0. repeat solve_incl.
+  Qed.
+
+  Fact normalize_reset_typeof_bool : forall e e' eqs' st st',
+      typeof e = [Op.bool_type] ->
+      normalize_reset e st = (e', eqs', st') ->
+      typeof e' = [Op.bool_type].
+  Proof.
+    intros e e' eqs' st st' Htyp Hnorm.
+    specialize (normalize_reset_spec e) as [[? [? [? Hspec]]]|Hspec]; subst;
+      rewrite Hspec in Hnorm; clear Hspec; repeat inv_bind.
+    - simpl in Htyp. assumption.
+    - destruct (hd _) eqn:Hann; simpl in *; repeat inv_bind;
+        destruct e; simpl in *; try solve [inv Hann; auto].
+      1,3,4: (destruct l1; try destruct l1; simpl in *; inv Hann; simpl in *; auto; destruct l1; congruence).
+      + destruct l0. destruct l0; simpl in *; inv Hann; simpl in *; auto.
+        destruct l0; congruence.
+      + destruct l0; try destruct a; simpl in *; inv Hann; simpl in *; auto.
+        destruct l0; congruence.
+  Qed.
+
+  Fact normalize_reset_wt_exp : forall G vars e e' eqs' st st',
+      wt_exp G (vars++(st_tys st)) e ->
+      normalize_reset e st = (e', eqs', st') ->
+      wt_exp G (vars++(st_tys st')) e'.
+  Proof.
+    intros G vars e e' eqs' st st' Hwt Hnorm.
+    specialize (normalize_reset_spec e) as [[? [? [? Hspec]]]|Hspec]; subst;
+      rewrite Hspec in Hnorm; clear Hspec; repeat inv_bind.
+    - assumption.
+    - destruct (hd _) eqn:Hann; simpl in *; repeat inv_bind.
+      constructor.
+      + unfold fresh_ident in H. destruct st as [n l]. inv H.
+        apply in_or_app. simpl. auto.
+      + apply fresh_ident_st_follows in H.
+        destruct e; simpl in Hann; inv Hann; inv Hwt.
+        1: repeat constructor.
+        1,2,3: (repeat solve_incl).
+        5,6: destruct l0; simpl in *; inv H1; repeat constructor; inv H9; repeat solve_incl.
+        2,3,4: destruct l; simpl in *; inv H1; repeat constructor.
+        1: destruct l1; simpl in *; inv H1; repeat constructor; inv H8; repeat solve_incl.
+        1: inv H5. 2: inv H5. 3: inv H6.
+        1,2,3: (destruct (map _) eqn:Hmap; simpl in *; inv H2; repeat constructor;
+              apply map_cons' in Hmap; destruct Hmap as [? [? [Hmap _]]]; inv Hmap; repeat solve_incl).
+  Qed.
+
+  Fact normalize_exp_wt_exp : forall G vars e is_control es' eqs' st st',
       wt_exp G vars e ->
       normalize_exp is_control e st = (es', eqs', st') ->
-      Forall (wt_exp G (vars++(idty (idty (snd st'))))) es'. (* non mauvais invariant *)
-  Proof.
+      Forall (wt_exp G (vars++(st_tys st'))) es'.
+  Proof with eauto.
     intros G vars e is_control es' eqs' st st' Hwt;
       revert is_control eqs' es' st st'.
     induction Hwt using wt_exp_ind2;
       intros is_control eqs' es' st st' Hnorm; simpl in *.
     - (* const *)
-      repeat inv_bind; eauto.
+      repeat inv_bind...
     - (* var *)
       repeat inv_bind.
       repeat constructor.
-      + apply in_or_app; auto.
-      + eapply wt_nclock_incl; eauto.
-        apply incl_appl. apply incl_refl.
+      + apply in_or_app...
+      + repeat solve_incl.
     - (* unop *)
       repeat inv_bind.
       specialize (IHHwt _ _ _ _ _ H2).
@@ -111,11 +402,10 @@ Module Type CORRECTNESS
       rewrite <- numstreams_length_typeof in Hlen.
       replace (typeof e) in *.
       singleton_length.
-      inv IHHwt. econstructor; eauto.
-      eapply normalize_exp_typeof in Hwt; eauto.
-      simpl in *; rewrite app_nil_r in Hwt; rewrite Hwt; auto.
-      eapply wt_nclock_incl; eauto.
-      apply incl_appl; apply incl_refl.
+      inv IHHwt. econstructor...
+      eapply normalize_exp_typeof in Hwt...
+      simpl in *; rewrite app_nil_r in Hwt; rewrite Hwt...
+      eapply wt_nclock_incl; [| eauto]...
     - (* binop *)
       repeat inv_bind.
       specialize (IHHwt1 _ _ _ _ _ H3).
@@ -128,95 +418,667 @@ Module Type CORRECTNESS
       replace (typeof e1) in *.
       replace (typeof e2) in *.
       repeat singleton_length.
-      eapply normalize_exp_typeof in Hwt1; eauto.
-      eapply normalize_exp_typeof in Hwt2; eauto.
+      eapply normalize_exp_typeof in Hwt1...
+      eapply normalize_exp_typeof in Hwt2...
       inv IHHwt1. inv IHHwt2. inv H8. inv H10.
       econstructor; eauto;
         simpl in *; rewrite app_nil_r in *;
-          try rewrite Hwt1; try rewrite Hwt2; auto.
-      + eapply wt_exp_incl; eauto.
-        apply incl_app.
-        * apply incl_appl; reflexivity.
-        * apply incl_appr. eapply st_follows_incl; eauto.
-      + eapply wt_nclock_incl; [| eauto].
-        apply incl_appl; reflexivity.
+          try rewrite Hwt1; try rewrite Hwt2...
+      + eapply normalize_exp_st_follows in H4. repeat solve_incl.
+      + repeat solve_incl.
     - (* fby *)
       repeat inv_bind.
-      admit.
+      specialize (idents_for_anns_incl _ _ _ _ H9) as Hincl.
+      apply idents_for_anns_wt with (G:=G) (vars:=vars) in H9.
+      + solve_forall.
+        eapply wt_exp_incl; [| eauto].
+        apply incl_app... apply incl_appr. apply incl_map...
+      + rewrite Forall_forall in *; intros.
+        destruct x as [? [? ?]]. eapply H5.
+        simpl_In.
+        exists (t, (c, o)); simpl...
     - (* when *)
       repeat inv_bind.
       specialize (map_bind2_normalize_exp_length _ _ _ _ _ _ _ _ H H1) as Hlength.
       specialize (map_bind2_normalize_exp_typeof _ _ _ _ _ _ _ _ H H1) as Htypeof.
-      admit.
-  Admitted.
+      repeat rewrite_Forall_forall.
+      rewrite in_map_iff in H4; destruct H4 as [[? ?] [? Hin]]; subst.
+      constructor; simpl...
+      + repeat constructor. eapply map_bind2_wt_exp in H1.
+        * rewrite Forall_forall in H1...
+        * intros; eapply normalize_exp_st_follows...
+        * rewrite Forall_forall; intros.
+          eapply H0 in H5; eauto.
+          solve_forall. repeat solve_incl.
+      + rewrite app_nil_r.
+        specialize (map_bind2_normalize_exp_numstreams _ _ _ _ _ _ H1) as Hnumstreams.
+        eapply map_bind2_normalize_exp_typeof in H1; [| rewrite Forall_forall; intros; auto].
+        rewrite <- Htypeof in Hin.
+        repeat simpl_nth.
+        unfold typesof. rewrite flat_map_concat_map.
+        eapply concat_length_map_nth; solve_forall.
+        * repeat solve_length.
+        * rewrite numstreams_length_typeof...
+      + apply in_or_app...
+      + repeat solve_incl.
+    - (* merge *)
+      destruct is_control; repeat inv_bind.
+      + rewrite Forall_forall; intros ? Hin.
+        rewrite in_map_iff in Hin; destruct Hin as [[[? ?] ?] [? Hin]]; subst.
+        specialize (map_bind2_normalize_exp_length _ _ _ _ _ _ _ _ H H7) as Hlength1.
+        specialize (map_bind2_normalize_exp_length _ _ _ _ _ _ _ _ H1 H4) as Hlength2.
+        constructor; simpl...
+        * eapply map_bind2_wt_exp with (G0:=G) (vars0 := (vars++(st_tys x2))) in H7...
+          -- apply map_bind2_st_follows in H4; solve_forall...
+             inv H8; [| inv H9].
+             repeat simpl_In.
+             rewrite Forall_forall in H7. apply H7 in H9.
+             repeat constructor. repeat solve_incl.
+          -- solve_forall. apply H8 in H9.
+             solve_forall. repeat solve_incl.
+        * eapply map_bind2_wt_exp with (G0:=G) (vars0 := (vars++(st_tys st'))) in H4...
+          -- repeat simpl_In.
+             rewrite Forall_forall in H4. apply H4 in H8.
+             repeat constructor. repeat solve_incl.
+          -- solve_forall. eapply H8 in H9.
+             solve_forall. repeat solve_incl.
+        * apply in_or_app...
+        * rewrite app_nil_r.
+          specialize (map_bind2_normalize_exp_numstreams _ _ _ _ _ _ H7) as Hnumstreams.
+          eapply map_bind2_normalize_exp_typeof in H7; [| rewrite Forall_forall in *; intros; auto].
+          rewrite <- H7 in Hin.
+          repeat simpl_nth.
+          unfold typesof. rewrite flat_map_concat_map.
+          eapply concat_length_map_nth; solve_forall.
+          -- repeat solve_length.
+          -- rewrite numstreams_length_typeof...
+        * rewrite app_nil_r.
+          specialize (map_bind2_normalize_exp_numstreams _ _ _ _ _ _ H4) as Hnumstreams.
+          eapply map_bind2_normalize_exp_typeof in H4; [| rewrite Forall_forall in *; intros; auto].
+          rewrite <- H5 in Hin. rewrite <- H4 in Hin.
+          repeat simpl_nth.
+          unfold typesof. rewrite flat_map_concat_map.
+          eapply concat_length_map_nth; solve_forall.
+          -- repeat solve_length.
+          -- rewrite numstreams_length_typeof...
+        * repeat solve_incl.
+      + specialize (idents_for_anns_incl _ _ _ _ H9) as Hincl.
+        apply idents_for_anns_wt with (G:=G) (vars:=vars) in H9.
+        * solve_forall. unfold st_tys. repeat solve_incl.
+        * rewrite Forall_forall; intros.
+          repeat simpl_In. inv H8...
+    - (* merge *)
+      destruct is_control; repeat inv_bind.
+      + rewrite Forall_forall; intros ? Hin.
+        rewrite in_map_iff in Hin; destruct Hin as [[[? ?] ?] [? Hin]]; subst.
+        specialize (map_bind2_normalize_exp_length _ _ _ _ _ _ _ _ H H8) as Hlength1.
+        specialize (map_bind2_normalize_exp_length _ _ _ _ _ _ _ _ H1 H4) as Hlength2.
+        constructor; simpl...
+        * apply IHHwt in H7.
+          apply hd_default_wt_exp. solve_forall.
+          apply map_bind2_st_follows in H8; solve_forall.
+          apply map_bind2_st_follows in H4; solve_forall.
+          repeat solve_incl.
+        * eapply map_bind2_wt_exp with (G0:=G) (vars0 := (vars++(st_tys x4))) in H8...
+          -- apply map_bind2_st_follows in H4; solve_forall...
+             inv H9; [| inv H10].
+             repeat simpl_In.
+             rewrite Forall_forall in H8. apply H8 in H10.
+             repeat constructor. repeat solve_incl.
+          -- solve_forall. apply H9 in H10.
+             solve_forall. repeat solve_incl.
+        * eapply map_bind2_wt_exp with (G0:=G) (vars0 := (vars++(st_tys st'))) in H4...
+          -- repeat simpl_In.
+             rewrite Forall_forall in H4. apply H4 in H9.
+             repeat constructor. repeat solve_incl.
+          -- solve_forall. eapply H9 in H10.
+             solve_forall. repeat solve_incl.
+        * specialize (normalize_exp_length _ _ _ _ _ _ _ _ Hwt H7) as Hlength.
+          rewrite <- numstreams_length_typeof in Hlength.
+          rewrite H3 in Hlength; simpl in Hlength.
+          eapply normalize_exp_typeof in H7...
+          destruct x; simpl in *; try congruence.
+          destruct x; simpl in *; try congruence.
+          rewrite app_nil_r in H7. congruence.
+        * rewrite app_nil_r.
+          specialize (map_bind2_normalize_exp_numstreams _ _ _ _ _ _ H8) as Hnumstreams.
+          eapply map_bind2_normalize_exp_typeof in H8; [| rewrite Forall_forall in *; intros; auto].
+          rewrite <- H8 in Hin.
+          repeat simpl_nth.
+          unfold typesof. rewrite flat_map_concat_map.
+          eapply concat_length_map_nth; solve_forall.
+          -- repeat solve_length.
+          -- rewrite numstreams_length_typeof...
+        * rewrite app_nil_r.
+          specialize (map_bind2_normalize_exp_numstreams _ _ _ _ _ _ H4) as Hnumstreams.
+          eapply map_bind2_normalize_exp_typeof in H4; [| rewrite Forall_forall in *; intros; auto].
+          rewrite <- H5 in Hin. rewrite <- H4 in Hin.
+          repeat simpl_nth.
+          unfold typesof. rewrite flat_map_concat_map.
+          eapply concat_length_map_nth; solve_forall.
+          -- repeat solve_length.
+          -- rewrite numstreams_length_typeof...
+        * repeat solve_incl.
+      + specialize (idents_for_anns_incl _ _ _ _ H10) as Hincl.
+        apply idents_for_anns_wt with (G:=G) (vars:=vars) in H10.
+        * solve_forall. unfold st_tys. repeat solve_incl.
+        * rewrite Forall_forall; intros.
+          destruct x2. repeat simpl_In. inv H9...
+    - (* app *)
+      repeat inv_bind.
+      specialize (idents_for_anns_incl _ _ _ _ H6) as Hincl.
+      apply idents_for_anns_wt with (G:=G) (vars:=vars) in H6.
+      + solve_forall. unfold st_tys. repeat solve_incl.
+      + rewrite Forall_forall in *; intros.
+        destruct x as [? [? ?]]. specialize (H4 _ H7); simpl in H4; eauto.
+    - (* app (reset) *)
+      repeat inv_bind.
+      specialize (idents_for_anns_incl _ _ _ _ H8) as Hincl.
+      apply idents_for_anns_wt with (G:=G) (vars:=vars) in H8.
+      + solve_forall. unfold st_tys. repeat solve_incl.
+      + rewrite Forall_forall in *; intros.
+        destruct x as [? [? ?]]. specialize (H4 _ H10); simpl in H4; eauto.
+  Qed.
+
+  Corollary map_bind2_normalize_exp_wt_exp : forall G vars is_control es es' eqs' st st',
+      Forall (wt_exp G vars) es ->
+      map_bind2 (normalize_exp is_control) es st = (es', eqs', st') ->
+      Forall (wt_exp G (vars++(st_tys st'))) (concat es').
+  Proof.
+    intros G vars is_control es es' eqs' st st' Hwt Hmap.
+    eapply map_bind2_wt_exp in Hmap; solve_forall; eauto.
+    eapply normalize_exp_wt_exp in H0; eauto.
+    solve_forall. repeat solve_incl.
+  Qed.
+
+  Corollary normalize_exps_wt_exp : forall G vars es es' eqs' st st',
+      Forall (wt_exp G vars) es ->
+      normalize_exps es st = (es', eqs', st') ->
+      Forall (wt_exp G (vars++(st_tys st'))) es'.
+  Proof.
+    intros G vars es es' eqs' st st' Hwt Hmap.
+    unfold normalize_exps in Hmap; repeat inv_bind.
+    eapply map_bind2_normalize_exp_wt_exp in H; eauto.
+  Qed.
+
+  Fact normalize_rhs_wt_exp : forall G vars e keep_fby es' eqs' st st',
+      wt_exp G vars e ->
+      normalize_rhs keep_fby e st = (es', eqs', st') ->
+      Forall (wt_exp G (vars++(st_tys st'))) es'.
+  Proof with eauto.
+    intros G vars e keep_fby es' eqs' st st' Hwt Hnorm.
+    destruct e; unfold normalize_rhs in Hnorm;
+      try (solve [eapply normalize_exp_wt_exp in Hnorm; eauto]).
+    - (* fby *)
+      destruct keep_fby.
+      + inv Hwt. repeat inv_bind.
+        eapply normalize_fby_wt_exp in H1; eauto.
+        * eapply normalize_exps_wt_exp in H; eauto.
+          solve_forall.
+          eapply normalize_exps_st_follows in H0.
+          eapply normalize_fby_st_follows in H1.
+          repeat solve_incl.
+        * eapply normalize_exps_wt_exp in H0; eauto.
+        * specialize (normalize_exps_length _ _ _ _ _ _ _ H2 H) as Hlength.
+          specialize (normalize_exps_numstreams _ _ _ _ _ H) as Hnumstreams.
+          unfold normalize_exps in H; repeat inv_bind.
+          eapply map_bind2_normalize_exp_typeof' in H; eauto.
+          assert (Forall2 (fun tys tys' => tys = tys') (map typesof x5) (map typeof l)).
+          { specialize (Forall2_map_1 (fun tys e => tys = typeof e) typesof x5 l) as [_ Hfm].
+            specialize (Forall2_map_2 (fun tys tys' => tys = tys') typeof (map typesof x5) l) as [_ Hfm2].
+            auto. } rewrite Forall2_eq in H7.
+          repeat rewrite_Forall_forall.
+          -- solve_length.
+          -- rewrite (concat_length_map_nth _ _ _ _ (fst b))...
+             ++ unfold typesof in *. rewrite flat_map_concat_map in H5. rewrite <- H7 in H5.
+              rewrite <- (map_nth fst). rewrite <- H5.
+             rewrite typeof_concat_typesof. reflexivity.
+             ++ solve_forall. rewrite numstreams_length_typeof...
+        * specialize (normalize_exps_length _ _ _ _ _ _ _ H3 H0) as Hlength.
+          specialize (normalize_exps_numstreams _ _ _ _ _ H0) as Hnumstreams.
+          unfold normalize_exps in H0; repeat inv_bind.
+          eapply map_bind2_normalize_exp_typeof' in H0; eauto.
+          assert (Forall2 (fun tys tys' => tys = tys') (map typesof x5) (map typeof l0)).
+          { specialize (Forall2_map_1 (fun tys e => tys = typeof e) typesof x5 l0) as [_ Hfm].
+            specialize (Forall2_map_2 (fun tys tys' => tys = tys') typeof (map typesof x5) l0) as [_ Hfm2].
+            auto. } rewrite Forall2_eq in H7.
+          repeat rewrite_Forall_forall.
+          -- solve_length.
+          -- rewrite (concat_length_map_nth _ _ _ _ (fst b))...
+             ++ unfold typesof in *. rewrite flat_map_concat_map in H4. rewrite <- H7 in H4.
+              rewrite <- (map_nth fst). rewrite <- H4.
+             rewrite typeof_concat_typesof. reflexivity.
+             ++ solve_forall. rewrite numstreams_length_typeof...
+        * rewrite Forall_map in H6. solve_forall. destruct a...
+      + eapply normalize_exp_wt_exp in Hnorm; eauto.
+    - (* app *)
+      inv Hwt; repeat inv_bind; repeat econstructor; eauto.
+      1,4: eapply normalize_exps_wt_exp...
+      2,4:solve_forall; repeat solve_incl.
+      + eapply normalize_exps_typesof in H... congruence.
+      + eapply normalize_exps_typesof in H0... congruence.
+      + eapply normalize_exp_wt_exp in H...
+        eapply hd_default_wt_exp in H.
+        eapply normalize_reset_wt_exp in H1...
+        apply normalize_exps_st_follows in H0.
+        repeat solve_incl.
+      + specialize (normalize_exp_numstreams _ _ _ _ _ _ H) as Hlength.
+        eapply normalize_exp_typeof in H...
+        eapply normalize_reset_typeof_bool in H1...
+        rewrite H9 in H.
+        destruct x4; simpl in *; try congruence.
+        inv Hlength. rewrite <- numstreams_length_typeof in H11.
+        destruct (typeof e); simpl in *; try congruence.
+        destruct l1; simpl in *; try congruence.
+  Qed.
+
+  Corollary normalize_rhss_wt_exp : forall G vars es keep_fby es' eqs' st st',
+      Forall (wt_exp G vars) es ->
+      normalize_rhss keep_fby es st = (es', eqs', st') ->
+      Forall (wt_exp G (vars++(st_tys st'))) es'.
+  Proof with eauto.
+    intros G vars es keep_fby es' eqs' st st' Hwt Hnorm.
+    unfold normalize_rhss in Hnorm; repeat inv_bind.
+    eapply map_bind2_wt_exp in H...
+    solve_forall.
+    eapply normalize_rhs_wt_exp in H1...
+    solve_forall. repeat solve_incl.
+  Qed.
 
   Fact map_bind2_wt_eq {A A1 B} :
     forall G vars (k : A -> Fresh (A1 * list equation) B) a a1s eqs' st st',
       map_bind2 k a st = (a1s, eqs', st') ->
-      Forall (fun a => forall a1 eqs' st st',
-                  k a st = (a1, eqs', st') ->
+      (forall st st' a es a2s, k a st = (es, a2s, st') -> fresh_st_follows st st') ->
+      Forall (fun a => forall a1 eqs' st0 st0',
+                  k a st0 = (a1, eqs', st0') ->
+                  fresh_st_follows st st0 ->
+                  fresh_st_follows st0' st' ->
                   Forall (wt_equation G vars) eqs') a ->
       Forall (wt_equation G vars) (concat eqs').
   Proof.
-    intros G vars k a a1s eqs' st st' Hmap Hf.
-    apply map_bind2_values in Hmap.
-    induction Hmap; inv Hf.
+   intros G vars k a.
+    induction a; intros es' a2s st st' Hmap Hfollows Hforall;
+      simpl in Hmap; repeat inv_bind.
     - constructor.
-    - simpl. apply Forall_app.
-      destruct H as [? [? H]].
-      split; eauto.
+    - apply Forall_app. split; eauto.
+      + rewrite Forall_forall in Hforall.
+        eapply Hforall; eauto.
+        * constructor. reflexivity.
+        * reflexivity.
+        * eapply map_bind2_st_follows in H0; eauto.
+          rewrite Forall_forall; intros; eauto.
+      + eapply IHa; eauto.
+        rewrite Forall_forall in *; intros.
+        eapply Hforall; eauto. apply in_cons; auto.
+        etransitivity; eauto.
   Qed.
 
-  (* Fact normalize_fby_wt_eq : forall G vars e0s es anns es' eqs' st st', *)
-  (*     normalize_fby e0s es anns st = (es', eqs', st') -> *)
-  (*     Forall (wt_equation G vars) eqs'. *)
-  (* Proof. *)
-  (*   intros G vars e0s es anns es' eqs' st st' Hnorm. *)
-  (*   unfold normalize_fby in Hnorm. repeat inv_bind. *)
-  (*   eapply map_bind2_wt_eq; eauto. *)
-  (*   rewrite Forall_forall; intros. destruct x as [[e0 e] [ty cl]]. *)
-  (*   specialize (fby_iteexp_spec e0 e ty cl) as [[c [? Hfby]]|Hfby]; subst; rewrite Hfby in H1; clear Hfby; *)
-  (*     repeat inv_bind. *)
-  (*   - constructor. *)
-  (*   - repeat constructor; simpl in *. *)
-  (* Admitted. *)
+  Fact add_whens_typeof : forall e ty cl,
+      typeof e = [ty] ->
+      typeof (add_whens e ty cl) = [ty].
+  Proof.
+    induction cl; intro Hty; simpl; auto.
+  Qed.
+
+  Fact add_whens_wt_exp : forall G vars e ty cl e',
+      wt_exp G vars e ->
+      typeof e = [ty] ->
+      wt_clock vars cl ->
+      add_whens e ty cl = e' ->
+      wt_exp G vars e'.
+  Proof.
+    induction cl; intros e' Hwt Hty Hclock Hwhens; simpl in Hwhens; inv Hclock; subst.
+    - assumption.
+    - repeat constructor; simpl; auto.
+      rewrite app_nil_r.
+      rewrite add_whens_typeof; auto.
+  Qed.
+
+  Fact normalize_fby_wt_eq : forall G vars e0s es anns es' eqs' st st',
+      Forall (wt_exp G (vars++(st_tys st))) e0s ->
+      Forall (wt_exp G (vars++(st_tys st))) es ->
+      Forall2 (fun e0 a => typeof e0 = [fst a]) e0s anns ->
+      Forall2 (fun e a => typeof e = [fst a]) es anns ->
+      Forall (fun '(_, cl) => wt_nclock vars cl) anns ->
+      normalize_fby e0s es anns st = (es', eqs', st') ->
+      Forall (wt_equation G (vars++(st_tys st'))) eqs'.
+  Proof with eauto.
+    intros G vars e0s es anns es' eqs' st st' Hwt1 Hwt2 Hty1 Hty2 Hclock Hnorm.
+    unfold normalize_fby in Hnorm. repeat inv_bind.
+    eapply map_bind2_wt_eq in H; eauto.
+    - intros; destruct a as [[e0 e] a]...
+    - repeat rewrite_Forall_forall. destruct x as [[e0 e] [ty cl]].
+      specialize (fby_iteexp_spec e0 e ty cl) as [[c [? Hspec]]|Hspec]; subst;
+        rewrite Hspec in H5; clear Hspec;
+          repeat inv_bind; inv H8.
+      + repeat constructor; simpl.
+        * repeat simpl_In.
+          apply Hwt2 in H8. repeat solve_incl.
+        * rewrite app_nil_r.
+          repeat simpl_nth. repeat simpl_length.
+          specialize (H1 _ _ _ _ _ H4 H13 H12); simpl in H1. congruence.
+        * f_equal. apply Op.type_init_type.
+        * repeat simpl_In.
+          apply Hclock in H4. repeat solve_incl.
+        * destruct x3; simpl in H9; inv H9.
+          apply st_follows_tys_incl in H7.
+          apply in_or_app; right.
+          apply H7. simpl...
+      + destruct st0; simpl in H5.
+        destruct (find _ _) eqn:Hfind; inv H5; [destruct p; inv H11|]; inv H10;
+          repeat constructor; simpl; try rewrite app_nil_r.
+        1,2: eapply add_whens_wt_exp; eauto; simpl.
+        5,6: rewrite add_whens_typeof; eauto; simpl.
+        1,6: f_equal; apply Op.type_true_const.
+        2,4: f_equal; apply Op.type_false_const.
+        1,2: repeat simpl_In; apply Hclock in H4; destruct cl; inv H4; simpl in *; repeat solve_incl.
+        * simpl_In. apply Hclock in H4. repeat solve_incl.
+        * apply fresh_ident_st_follows in H9. apply st_follows_tys_incl in H9.
+          apply st_follows_tys_incl in H7.
+          apply in_or_app. right. apply H7. apply H9.
+          simpl...
+        * inv H5.
+  Qed.
+
+  Fact normalize_reset_wt_eq : forall G vars e e' eqs' st st',
+      wt_exp G (vars++(st_tys st)) e ->
+      typeof e = [Op.bool_type] ->
+      normalize_reset e st = (e', eqs', st') ->
+      Forall (wt_equation G (vars++(st_tys st'))) eqs'.
+  Proof.
+    intros G vars e e' eqs' st st' Hwt Hty Hnorm.
+    specialize (normalize_reset_spec e) as [[? [? [? Hspec]]]|Hspec]; subst;
+      rewrite Hspec in Hnorm; clear Hspec; repeat inv_bind.
+    - constructor.
+    - destruct (hd _) eqn:Hann; simpl in *. repeat inv_bind.
+      repeat constructor; simpl.
+      + repeat solve_incl.
+      + rewrite app_nil_r. rewrite Hty.
+        repeat constructor.
+        unfold fresh_ident in H.
+        destruct st. inv H.
+        apply in_or_app; simpl. right. left.
+        f_equal.
+        destruct (annot e) eqn:Hannot; simpl in Hann; inv Hann. reflexivity.
+        destruct e; simpl in *; inv Hannot; inv Hty; auto;
+          try destruct l2; try destruct l3; simpl in *; subst; inv H0; reflexivity.
+  Qed.
 
   Fact normalize_exp_wt_eq : forall G vars e is_control es' eqs' st st',
       wt_exp G vars e ->
       normalize_exp is_control e st = (es', eqs', st') ->
-      Forall (wt_equation G vars (* FIXME *)) eqs'.
-  Proof.
+      Forall (wt_equation G (vars++(st_tys st'))) eqs'.
+  Proof with eauto.
     induction e using exp_ind2; intros is_control es' eqs' st st' Hwt Hnorm;
-      inv Hwt; simpl in Hnorm; repeat inv_bind.
+      simpl in Hnorm; repeat inv_bind.
     - (* const *) constructor.
     - (* var *) constructor.
-    - (* unop *) eauto.
+    - (* unop *) inv Hwt...
     - (* binop *)
+      inv Hwt.
       rewrite Forall_app.
       split; eauto.
+      eapply IHe1 in H; eauto.
+      solve_forall. eapply wt_equation_incl; [| eauto].
+      eapply normalize_exp_st_follows in H0.
+      repeat solve_incl.
     - (* fby *)
+      inv Hwt.
       repeat rewrite Forall_app.
-      repeat split; eauto;
-        try (eapply map_bind2_wt_eq; eauto;
-             rewrite Forall_forall in *;
-             intros; eauto).
-      admit. admit.
+      repeat split; eauto.
+      + solve_forall. destruct x.
+        repeat constructor.
+        * repeat simpl_In. inv H5. repeat constructor.
+          eapply normalize_fby_wt_exp with (G:=G) (vars:=vars) in H3...
+          -- rewrite Forall_forall in H3...
+             apply H3 in H6. repeat solve_incl.
+          -- eapply map_bind2_normalize_exp_wt_exp in H1...
+             solve_forall. repeat solve_incl.
+          -- eapply map_bind2_normalize_exp_wt_exp in H2...
+          -- admit.
+          -- admit.
+          -- rewrite Forall_forall in *; intros [ty cl] Hin.
+             apply H12. repeat simpl_In. exists (ty, cl)...
+        * specialize (normalize_fby_numstreams _ _ _ _ _ _ _ H3) as Hnumstreams. rewrite Forall_forall in Hnumstreams.
+          repeat simpl_In. inv H5. simpl. rewrite app_nil_r.
+          specialize (Hnumstreams _ H6). rewrite <- numstreams_length_typeof in Hnumstreams.
+          remember (typeof e) as ts.
+          singleton_length. repeat constructor.
+          apply idents_for_anns_values in H4.
+          apply normalize_fby_typeof in H3; admit. (* penible *)
+      + eapply map_bind2_wt_eq in H1; eauto.
+        rewrite Forall_forall in *; intros.
+        specialize (H _ H5 _ _ _ _ _ (H8 _ H5) H6).
+        solve_forall. repeat solve_incl.
+      + eapply map_bind2_wt_eq in H2; eauto.
+        rewrite Forall_forall in *; intros.
+        specialize (H0 _ H5 _ _ _ _ _ (H9 _ H5) H6).
+        solve_forall. repeat solve_incl.
+      + eapply normalize_fby_wt_eq with (G:=G) (vars:=vars) in H3...
+        * solve_forall. repeat solve_incl.
+        * eapply map_bind2_normalize_exp_wt_exp in H1...
+          solve_forall. repeat solve_incl.
+        * eapply map_bind2_normalize_exp_wt_exp in H2...
+        * admit.
+        * admit.
+        * rewrite Forall_forall in *; intros [ty cl] Hin.
+          apply H12. repeat simpl_In. exists (ty, cl)...
     - (* when *)
+      inv Hwt; repeat inv_bind.
       eapply map_bind2_wt_eq; eauto.
-      rewrite Forall_forall in *; intros; eauto.
+      rewrite Forall_forall in *; intros.
+      eapply H in H2; eauto.
+      solve_forall.
+      eapply wt_equation_incl; [| eauto]. repeat solve_incl.
     - (* merge *)
+      inv Hwt.
       destruct is_control; repeat inv_bind.
-      + (* exp *)
-        apply Forall_app; split;
-          (eapply map_bind2_wt_eq; eauto;
-           rewrite Forall_forall in *; intros; eauto).
       + (* control *)
-        repeat rewrite Forall_app.
-        repeat split;
-          try (eapply map_bind2_wt_eq; eauto;
-               rewrite Forall_forall in *; intros; eauto).
-        admit.
+        apply Forall_app; split.
+        * eapply map_bind2_wt_eq in H1; eauto.
+          rewrite Forall_forall in *; intros.
+          eapply H in H4; eauto.
+          solve_forall. repeat solve_incl.
+        * eapply map_bind2_wt_eq in H2; eauto.
+          rewrite Forall_forall in *; intros.
+          eapply H0 in H4; eauto.
+          solve_forall. repeat solve_incl.
+      + (* exp *)
+        repeat rewrite Forall_app; repeat split.
+        * solve_forall.
+          destruct x0 as [xs es].
+          repeat constructor; [repeat simpl_In |]; repeat constructor; simpl.
+          -- eapply map_bind2_normalize_exp_wt_exp in H1; eauto.
+             rewrite Forall_forall in H1. eapply H1 in H12.
+             eapply map_bind2_st_follows in H2; solve_forall.
+             repeat solve_incl.
+          -- eapply map_bind2_normalize_exp_wt_exp in H2; eauto.
+             rewrite Forall_forall in H2. eapply H2 in H4.
+             eapply idents_for_anns_st_follows in H3.
+             repeat solve_incl.
+          -- apply in_or_app...
+          -- rewrite app_nil_r. admit.
+          -- rewrite app_nil_r. admit.
+          -- repeat solve_incl.
+          -- admit. (* penible *)
+        * eapply map_bind2_wt_eq in H1; eauto.
+          rewrite Forall_forall in *; intros.
+          eapply H in H4; [| eauto | eauto].
+          solve_forall. repeat solve_incl.
+        * eapply map_bind2_wt_eq in H2; eauto.
+          rewrite Forall_forall in *; intros.
+          eapply H0 in H4; [| eauto | eauto].
+          solve_forall. repeat solve_incl.
+    - (* ite *) admit.
+    - (* app *)
+      inv Hwt; repeat inv_bind; repeat econstructor; simpl; eauto.
+      1,6: (eapply map_bind2_wt_exp with (vars0:=(vars++(st_tys st'))) in H2; eauto;
+            solve_forall;
+            try eapply normalize_exp_wt_exp in H4; try eapply normalize_exp_wt_exp in H6; eauto;
+            solve_forall; repeat solve_incl).
+      1,5: eapply map_bind2_normalize_exp_typeof in H2; eauto; congruence.
+      1,4: (solve_forall; repeat solve_incl).
+      1,5: rewrite app_nil_r.
+      + clear H0 H8 H10 H11 H12.
+        specialize (idents_for_anns_incl _ _ _ _ H3) as Hincl.
+        apply idents_for_anns_values in H3.
+        repeat rewrite_Forall_forall; repeat rewrite map_length in *...
+        apply in_or_app. right.
+        rewrite <- H0 in H3.
+        specialize (H1 (b, (Cbase, None)) (a0, (b, (Cbase, None))) _ _ _ H3 eq_refl eq_refl).
+        destruct (nth _ _ _) eqn:Hnth; subst.
+        erewrite map_nth'. 2: congruence.
+        rewrite H0 in H3. eapply nth_In in H3.
+        rewrite Hnth in *; simpl.
+        unfold st_tys. eapply Hincl in H3...
+        unfold idty. repeat simpl_In.
+        eexists; split; eauto; simpl. f_equal.
+        replace b with (fst (b, (Cbase, @None ident))) by reflexivity.
+        rewrite map_nth; reflexivity.
+      + clear H H0 H8 H10 H11 H12.
+        specialize (idents_for_anns_incl _ _ _ _ H3) as Hincl.
+        apply idents_for_anns_values in H3.
+        repeat rewrite_Forall_forall; repeat rewrite map_length in *...
+        apply in_or_app. right.
+        rewrite <- H in H3.
+        specialize (H0 (b, (Cbase, None)) (a0, (b, (Cbase, None))) _ _ _ H3 eq_refl eq_refl).
+        destruct (nth _ _ _) eqn:Hnth; subst.
+        erewrite map_nth'. 2: congruence.
+        rewrite H in H3. eapply nth_In in H3.
+        rewrite Hnth in *; simpl.
+        unfold st_tys. eapply Hincl in H3...
+        unfold idty. repeat simpl_In.
+        eexists; split; eauto; simpl. f_equal.
+        replace b with (fst (b, (Cbase, @None ident))) by reflexivity.
+        rewrite map_nth; reflexivity.
+      + eapply map_bind2_wt_eq in H2; eauto.
+        rewrite Forall_forall in *; intros.
+        eapply H0 in H4; eauto.
+        solve_forall. repeat solve_incl.
+      + eapply normalize_exp_wt_exp in H1...
+        eapply hd_default_wt_exp in H1...
+        eapply normalize_reset_wt_exp in H4...
+        eapply map_bind2_st_follows in H2; solve_forall.
+        repeat solve_incl.
+      + specialize (normalize_exp_numstreams _ _ _ _ _ _ H1) as Hlength.
+        eapply normalize_exp_typeof in H1...
+        eapply normalize_reset_typeof_bool in H4...
+        rewrite H14 in H1.
+        destruct x2; simpl in *; try congruence.
+        inv Hlength. rewrite <- numstreams_length_typeof in H7.
+        destruct (typeof e); simpl in *; try congruence.
+        destruct l; simpl in *; try congruence.
+      + repeat rewrite Forall_app. repeat split.
+        * eapply H in H1...
+          apply normalize_reset_st_follows in H4.
+          apply map_bind2_st_follows in H2; solve_forall.
+          apply idents_for_anns_st_follows in H3.
+          solve_forall. repeat solve_incl.
+        * specialize (normalize_exp_length _ _ _ _ _ _ _ _ H13 H1) as Hlength.
+          specialize (normalize_exp_typeof _ _ _ _ _ _ _ _ H13 H1) as Htypeof.
+          rewrite H14 in Htypeof.
+          eapply normalize_exp_wt_exp in H1... eapply hd_default_wt_exp in H1...
+          eapply normalize_reset_wt_eq in H4...
+          -- solve_forall. repeat solve_incl.
+          -- rewrite <- numstreams_length_typeof in Hlength. rewrite H14 in Hlength.
+             destruct x2; simpl in *; try congruence.
+             destruct x2; simpl in *; try congruence.
+             rewrite app_nil_r in Htypeof...
+        * eapply map_bind2_wt_eq in H2; eauto.
+          rewrite Forall_forall in *; intros.
+          eapply H0 in H6...
+          solve_forall. repeat solve_incl.
   Admitted.
+
+  Fact normalize_rhs_wt_eq : forall G vars e keep_fby es' eqs' st st',
+      wt_exp G vars e ->
+      normalize_rhs keep_fby e st = (es', eqs', st') ->
+      Forall (wt_equation G (vars++(st_tys st'))) eqs'.
+  Proof with eauto.
+    intros G vars e keep_fby es' eqs' st st' Hwt Hnorm.
+    destruct e; unfold normalize_rhs in Hnorm;
+      try eapply normalize_exp_wt_eq in Hnorm; eauto;
+        [destruct keep_fby|].
+    - (* fby *) admit.
+    - eapply normalize_exp_wt_eq...
+    - (* app *) admit.
+  Admitted.
+
+  Corollary normalize_rhss_wt_eq : forall G vars es keep_fby es' eqs' st st',
+      Forall (wt_exp G vars) es ->
+      normalize_rhss keep_fby es st = (es', eqs', st') ->
+      Forall (wt_equation G (vars++(st_tys st'))) eqs'.
+  Proof with eauto.
+    intros G vars es keep_fby es' eqs' st st' Hwt Hnorm.
+    unfold normalize_rhss in Hnorm; repeat inv_bind.
+    eapply map_bind2_wt_eq in H...
+    solve_forall. eapply normalize_rhs_wt_eq in H1...
+    solve_forall. repeat solve_incl.
+  Qed.
+
+  Fact normalize_equation_wt_eq : forall G vars eq to_cut eqs' st st',
+      wt_equation G vars eq ->
+      normalize_equation to_cut eq st = (eqs', st') ->
+      Forall (wt_equation G (vars++(st_tys st'))) eqs'.
+  Proof with eauto.
+    intros G vars eq to_cut eqs' st st' Hwt Hnorm.
+    destruct eq as [xs es]; simpl in Hnorm.
+    repeat inv_bind. destruct Hwt.
+    apply Forall_app. split.
+    - specialize (normalize_rhss_typeof _ _ _ _ _ _ _ _ H0 H) as Htypeof.
+      eapply normalize_rhss_wt_exp in H...
+      rewrite <- Htypeof in H1.
+      clear Htypeof. revert xs H1.
+      induction x; intros xs H1; constructor; simpl in H1.
+      + inv H. repeat constructor...
+        simpl. rewrite app_nil_r.
+        repeat rewrite_Forall_forall.
+        * admit.
+        * rewrite firstn_length in H2.
+          rewrite PeanoNat.Nat.min_glb_lt_iff in H2; destruct H2 as [_ H2].
+          admit.
+      + inv H. apply IHx...
+        admit.
+    - eapply normalize_rhss_wt_eq in H...
+  Admitted.
+
+  Corollary normalize_equations_wt_eq : forall G vars eqs to_cut eqs' st st',
+      Forall (wt_equation G vars) eqs ->
+      normalize_equations to_cut eqs st = (eqs', st') ->
+      Forall (wt_equation G (vars++(st_tys st'))) eqs'.
+  Proof with eauto.
+    induction eqs; intros to_cut eqs' st st' Hwt Hnorm;
+      simpl in Hnorm; repeat inv_bind.
+    - constructor.
+    - inv Hwt. apply Forall_app. split...
+      eapply normalize_equation_wt_eq in H...
+      solve_forall. repeat solve_incl.
+  Qed.
+
+  Lemma normalize_node_wt : forall n G Hwt n',
+      normalize_node n (ex_intro _ G Hwt) = n' ->
+      wt_node G n'.
+  Proof.
+    intros n G Hwt n' Hnorm. simpl in Hwt.
+    unfold normalize_node in Hnorm. subst.
+    destruct Hwt as [Hclin [Hclout [Hclvars Heq]]].
+    repeat constructor; simpl; auto.
+    - admit. (* wt_clocks hum... *)
+    - remember (normalize_equations (map fst (n_out n)) (n_eqs n) (first_unused_ident n, [])) as res.
+      destruct res as [eqs' st']; simpl.
+      symmetry in Heqres.
+      eapply normalize_equations_wt_eq in Heqres; eauto.
+      solve_forall. repeat solve_incl. clear Heqres H.
+      unfold st_tys, idty in *. apply incl_app.
+      + apply incl_map. apply incl_app; [solve_incl|].
+        apply incl_app; [| repeat solve_incl].
+        apply incl_appr. apply incl_appl; solve_incl.
+      + repeat rewrite map_map; simpl.
+        repeat rewrite map_app; simpl.
+        apply incl_appr. apply incl_appl. apply incl_appr.
+        repeat rewrite map_map; simpl. reflexivity.
+  Admitted.
+
 End CORRECTNESS.
 
 Module CorrectnessFun
